\documentclass{article}
\usepackage{amsmath}

\begin{document}
$$
A = 
\oint \int\limits_R dxdy = 
\int\limits_{-2a}^{a}\left[\int\limits_{y-a}^{a-\frac{y^2}{a}} dx\right] dy = 
\int\limits_{-2a}^{a}\left[\left.{x}\right|_{y-a}^{a-\frac{y^2}{a}}\right] dy =
\int\limits_{-2a}^{a}\left[a - \frac{y^2}{a} - (y-a)\right] dy =
$$

$$
=\int\limits_{-2a}^{a}\left(2a - \frac{y^2}{a} - y\right) dy =
\left.\left[2ay - \frac{y^3}{3a} - \frac{y^2}{2}\right]\right|_{-2a}^{a} =
\left(2a^2-\frac{a^3}{3a}-\frac{a^2}{2}\right)-\left(-4a^2+\frac{8a^3}{3a}-\frac{4a^2}{2}\right)=
\frac{9a^2}{2}
$$





\begin{equation}
\begin{gathered}
A =
\oint \int\limits_R dxdy = 
\int\limits_{-2a}^{a}\left[\int\limits_{y-a}^{a-\frac{y^2}{a}} dx\right] dy = 
\int\limits_{-2a}^{a}\left[\left.{x}\right|_{y-a}^{a-\frac{y^2}{a}}\right] dy =
\int\limits_{-2a}^{a}\left[a - \frac{y^2}{a} - (y-a)\right] dy =\\
=\int\limits_{-2a}^{a}\left(2a - \frac{y^2}{a} - y\right) dy =
\left.\left[2ay - \frac{y^3}{3a} - \frac{y^2}{2}\right]\right|_{-2a}^{a} =
\left(2a^2-\frac{a^3}{3a}-\frac{a^2}{2}\right)-\left(-4a^2+\frac{8a^3}{3a}-\frac{4a^2}{2}\right)=
\frac{9a^2}{2}
\end{gathered}
\end{equation}
\end{document}
